Invariant proposal for store. It seems sufficient for all operations except [store_restore]. Next step is to make the physical graph explicit, including captured nodes and diff nodes. Is the historical graph needed now?

theories/store.v
@@ -2,6 +2,9 @@
    https://gitlab.com/basile.clement/store/-/blob/main/src/store.ml?ref_type=heads
 *)
 
+From iris.base_logic Require Import
+  lib.ghost_map.
+
 From zebre Require Import
   prelude.
 From zebre.language Require Import
@@ -13,24 +16,20 @@ From zebre.std Require Import
 From zebre Require Import
   options.
 
-Implicit Types r : loc.
-Implicit Types v t s : val.
-Implicit Types σ : gmap loc val.
-
-#[local] Notation "'root'" := (
+#[local] Notation "'gen'" := (
   annotate "t" 0
 )(in custom zebre_field
 ).
-#[local] Notation "'gen'" := (
+#[local] Notation "'root'" := (
   annotate "t" 1
 )(in custom zebre_field
 ).
 
-#[local] Notation "'ref_value'" := (
+#[local] Notation "'ref_gen'" := (
   annotate "ref" 0
 )(in custom zebre_field
 ).
-#[local] Notation "'ref_gen'" := (
+#[local] Notation "'ref_value'" := (
   annotate "ref" 1
 )(in custom zebre_field
 ).
@@ -39,11 +38,11 @@ Implicit Types σ : gmap loc val.
   ("snap", 0)
 ( in custom zebre_proj
 ).
-#[local] Notation "'snap_root'" :=
+#[local] Notation "'snap_gen'" :=
   ("snap", 1)
 ( in custom zebre_proj
 ).
-#[local] Notation "'snap_gen'" :=
+#[local] Notation "'snap_root'" :=
   ("snap", 2)
 ( in custom zebre_proj
 ).
@@ -59,11 +58,11 @@ Implicit Types σ : gmap loc val.
 
 Definition store_create : val :=
   λ: <>,
-    { ref §Root; #0 }.
+    { #0; ref §Root }.
 
 Definition store_ref : val :=
   λ: "t" "v",
-    { "v"; #0 }.
+    { #0; "v" }.
 
 Definition store_get : val :=
   λ: "t" "r",
@@ -71,57 +70,23 @@ Definition store_get : val :=
 
 Definition store_set : val :=
   λ: "t" "r" "v",
-    let: "t_gen" := "t".{gen} in
-    let: "r_gen" := "r".{ref_gen} in
-    if: "t_gen" = "r_gen" then (
+    let: "g_t" := "t".{gen} in
+    let: "g_r" := "r".{ref_gen} in
+    if: "g_t" = "g_r" then (
       "r" <-{ref_value} "v"
     ) else (
       let: "root" := ref §Root in
-      "t".{root} <- ‘Diff{ "r", "r".{ref_value}, "r_gen", "root" } ;;
+      "t".{root} <- ‘Diff{ "r", "g_r", "r".{ref_value}, "root" } ;;
+      "r" <-{ref_gen} "g_t" ;;
       "r" <-{ref_value} "v" ;;
-      "r" <-{ref_gen} "t_gen" ;;
       "t" <-{root} "root"
     ).
 
 Definition store_capture : val :=
   λ: "t",
-    let: "gen" := "t".{gen} in
-    "t" <-{gen} #1 + "gen" ;;
-    ("t", "t".{root}, "gen").
-
-#[local] Definition store_reroot : val :=
-  rec: "store_reroot" "node" :=
-    match: !"node" with
-    | Root =>
-        ()
-    | Diff "r" "v" "gen" "node'" =>
-        "store_reroot" "node'" ;;
-        "node'" <- ‘Diff{ "r", "r".{ref_value}, "r".{ref_gen}, "node" } ;;
-        "r" <-{ref_value} "v" ;;
-        "r" <-{ref_gen} "gen" ;;
-        "node" <- §Root
-    end.
-
-#[local] Definition store_reroot_opt_aux : val :=
-  rec: "store_reroot_opt_aux" "node" :=
-    match: !"node" with
-    | Root =>
-        ()
-    | Diff "r" "v" "gen" "node'" =>
-        "store_reroot_opt_aux" "node'" ;;
-        "node'" <- ‘Diff{ "r", "r".{ref_value}, "r".{ref_gen}, "node" } ;;
-        "r" <-{ref_value} "v" ;;
-        "r" <-{ref_gen} "gen"
-    end.
-#[local] Definition store_reroot_opt : val :=
-  λ: "node",
-    match: !"node" with
-    | Root =>
-        ()
-    | Diff <> <> <> <> =>
-        store_reroot_opt_aux "node" ;;
-        "node" <- §Root
-    end.
+    let: "g" := "t".{gen} in
+    "t" <-{gen} #1 + "g" ;;
+    ("t", "g", "t".{root}).
 
 #[local] Definition store_collect : val :=
   rec: "store_collect" "node" "acc" :=
@@ -140,15 +105,15 @@ Definition store_capture : val :=
         match: !"node'" with
         | Root =>
             Fail
-        | Diff "r" "v" "gen" "node_" =>
+        | Diff "r" "v" "g" "node_" =>
             assert ("node_" = "node") ;;
-            "node" <- ‘Diff{ "r", "r".{ref_value}, "r".{ref_gen}, "node'" } ;;
+            "node" <- ‘Diff{ "r", "r".{ref_gen}, "r".{ref_value}, "node'" } ;;
+            "r" <-{ref_gen} "g" ;;
             "r" <-{ref_value} "v" ;;
-            "r" <-{ref_gen} "gen" ;;
             "store_revert" "node'" "seg"
         end
     end.
-#[local] Definition store_reroot_opt2 : val :=
+#[local] Definition store_reroot : val :=
   λ: "node",
     let: "collect" := store_collect "node" §Nil in
     store_revert "collect".<0> "collect".<1>.
@@ -164,15 +129,35 @@ Definition store_restore : val :=
           ()
       | Diff <> <> <> <> =>
           store_reroot "root" ;;
-          "t" <-{root} "root" ;;
-          "t" <-{gen} #1 + "s".<snap_gen>
+          "t" <-{gen} #1 + "s".<snap_gen> ;;
+          "t" <-{root} "root"
       end
     ).
 
+Implicit Types l r node cnode base root dst : loc.
+Implicit Types nodes : list loc.
+Implicit Types v t s : val.
+Implicit Types σ : gmap loc val.
+
+#[local] Definition generation :=
+  nat.
+Implicit Types g : generation.
+
+#[local] Definition store :=
+  gmap loc (generation * val).
+Implicit Types ς : store.
+Implicit Types data : generation * val.
+
+#[local] Definition descriptor : Set :=
+  generation * store.
+Implicit Types descr base_descr : descriptor.
+
 Class StoreG Σ `{zebre_G : !ZebreG Σ} := {
+  #[local] store_G_nodes_G :: ghost_mapG Σ loc descriptor ;
 }.
 
 Definition store_Σ := #[
+  ghost_mapΣ loc descriptor
 ].
 Lemma subG_store_Σ Σ `{zebre_G : !ZebreG Σ} :
   subG store_Σ Σ →
@@ -184,14 +169,78 @@ Qed.
 Section store_G.
   Context `{store_G : StoreG Σ}.
 
-  Definition store_store σ0 σ :=
-    union_with (λ _, Some) σ0 σ.
+  #[local] Definition store_on σ0 ς :=
+    ς ∪ (pair 0 <$> σ0).
+  #[local] Definition store_generation g ς :=
+    map_Forall (λ r data, data.1 ≤ g) ς.
 
-  Definition store_model t σ0 σ : iProp Σ.
-  Proof. Admitted.
+  #[local] Definition delta : Set :=
+    loc * (generation * val).
+  Implicit Types δ : delta.
+  Implicit Types δs : list delta.
 
-  Definition store_snapshot_model s t σ : iProp Σ.
-  Proof. Admitted.
+  #[local] Definition delta_apply δs ς :=
+    list_to_map δs ∪ ς.
+  #[local] Fixpoint delta_chain node nodes δs dst : iProp Σ :=
+    match nodes, δs with
+    | [], [] =>
+        ⌜node = dst⌝
+    | node' :: nodes, δ :: δs =>
+        node ↦ ’Diff{ #δ.1, #δ.2.1, δ.2.2, #node' } ∗
+        delta_chain node' nodes δs dst
+    | _, _ =>
+        False
+    end.
+
+  #[local] Definition cnodes_auth γ cnodes :=
+    ghost_map_auth γ 1 cnodes.
+  #[local] Definition cnodes_pointsto γ cnode descr :=
+    ghost_map_elem γ cnode (DfracOwn 1) descr.
+  #[local] Definition cnodes_elem γ cnode descr :=
+    ghost_map_elem γ cnode DfracDiscarded descr.
+
+  #[local] Definition cnode_model γ σ0 cnode descr node ς : iProp Σ :=
+    ⌜dom descr.2 ⊆ dom σ0⌝ ∗
+    ⌜store_generation descr.1 descr.2⌝ ∗
+    cnodes_elem γ cnode descr ∗
+    ( ∃ nodes δs,
+      ⌜store_on σ0 descr.2 = store_on σ0 $ delta_apply δs ς⌝ ∗
+      delta_chain cnode nodes δs node
+    ).
+  Definition store_model t σ0 σ : iProp Σ :=
+    ∃ l γ g root ς,
+    ⌜t = #l⌝ ∗
+    ⌜σ = snd <$> ς⌝ ∗
+    meta l nroot γ ∗
+    l.[gen] ↦ #g ∗
+    l.[root] ↦ #root ∗
+    root ↦ §Root ∗
+    ( [∗ map] r ↦ data ∈ store_on σ0 ς,
+      r.[ref_gen] ↦ #data.1 ∗
+      r.[ref_value] ↦ data.2
+    ) ∗
+    if g is 0 then
+      cnodes_pointsto γ root (0, ς)
+    else
+      ∃ cnodes base base_descr,
+      cnodes_auth γ cnodes ∗
+      (* base cnode *)
+      ⌜cnodes !! base = Some base_descr⌝ ∗
+      ⌜base_descr.1 < g⌝ ∗
+      cnode_model γ σ0 base base_descr root ς ∗
+      (* other cnodes *)
+      ( [∗ map] cnode ↦ descr ∈ delete base cnodes,
+        ∃ cnode' descr',
+        ⌜cnodes !! cnode' = Some descr'⌝ ∗
+        cnode_model γ σ0 cnode descr cnode' descr'.2
+      ).
+
+  Definition store_snapshot_model s t σ : iProp Σ :=
+    ∃ l γ g node descr,
+    ⌜t = #l ∧ s = (t, #g, #node)%V⌝ ∗
+    meta l nroot γ ∗
+    cnodes_elem γ node descr ∗
+    ⌜descr.1 ≤ g⌝.
 
   #[global] Instance store_model_timeless t σ0 σ :
     Timeless (store_model t σ0 σ).
@@ -200,7 +249,18 @@ Section store_G.
   #[global] Instance store_snapshot_persistent s t σ :
     Persistent (store_snapshot_model s t σ).
   Proof.
-  Abort.
+    apply _.
+  Qed.
+
+  #[local] Definition cnodes_alloc root :
+    ⊢ |==>
+      ∃ γ,
+      cnodes_auth γ {[root := (0, ∅)]} ∗
+      cnodes_pointsto γ root (0, ∅).
+  Proof.
+    iMod ghost_map_alloc as "(%γ & Hcnodes_auth & Hcnodes_pointsto)".
+    iSteps. rewrite big_sepM_singleton. iSteps.
+  Qed.
 
   Lemma store_create_spec :
     {{{ True }}}
@@ -210,7 +270,15 @@ Section store_G.
       store_model t ∅ ∅
     }}}.
   Proof.
-  Abort.
+    iIntros "%Φ _ HΦ".
+    wp_rec.
+    wp_alloc root as "Hroot".
+    wp_record l as "Hmeta" "(Hl_gen & Hl_root & _)".
+    iMod (cnodes_alloc root) as "(%γ & Hcnodes_auth & Hcnodes_pointsto)".
+    iMod (meta_set with "Hmeta") as "Hmeta"; first done.
+    iApply "HΦ".
+    iExists l, γ, 0, root, ∅. iFrame. rewrite big_sepM_empty. iSteps.
+  Qed.
 
   Lemma store_ref_spec t σ0 σ v :
     {{{
@@ -219,13 +287,14 @@ Section store_G.
       store_ref t v
     {{{ r,
       RET #r;
+      ⌜σ0 !! r = None⌝ ∗
       store_model t (<[r := v]> σ0) σ
     }}}.
   Proof.
   Abort.
 
   Lemma store_get_spec {t σ0 σ r} v :
-    store_store σ0 σ !! r = Some v →
+    (σ ∪ σ0) !! r = Some v →
     {{{
       store_model t σ0 σ
     }}}
@@ -250,7 +319,7 @@ Section store_G.
   Proof.
   Abort.
 
-  Lemma store_catpure_spec t σ0 σ :
+  Lemma store_capture_spec t σ0 σ :
     {{{
       store_model t σ0 σ
     }}}
